impHeap.lean
@@ -17,117 +17,117 @@ def ident := ℕ
 
 def env := ident → ℕ
 
-def empty_env (x : ℕ) := 0
+instance : inhabited env := ⟨λ x, 0⟩
+instance : inhabited heap := ⟨λ h, none⟩
+instance : inhabited cell := ⟨none⟩
 
-def empty_heap (h : ℕ) := @none ℕ
-
-def empty_cell := @none ℕ
+def empty_env : env := inhabited.default env
+def empty_heap : heap := inhabited.default heap
+def empty_cell : cell := inhabited.default cell
 
 def imp_state := heap × env
 
-def beq_nat : ℕ → ℕ → bool
-| 0 0 := tt
-| (x+1) (y+1) := (beq_nat x y)
-| (x+1) 0 := ff
-| 0 (x+1) := ff
+--def beq_nat : ℕ → ℕ → bool
+--| 0 0 := tt
+--| (x+1) (y+1) := (beq_nat x y)
+--| (x+1) 0 := ff
+--| 0 (x+1) := ff
 
-def ble_nat : ℕ → ℕ → bool
-| 0 z := tt
-| (x+1) (y+1) := (ble_nat x y)
-| (x+1) 0 := ff
+--def ble_nat : ℕ → ℕ → bool
+--| 0 z := tt
+--| (x+1) (y+1) := (ble_nat x y)
+--| (x+1) 0 := ff
 
-example : beq_nat 3 3=tt := rfl.
+--example : beq_nat 3 3=tt := rfl.
 
-def beq_ident := beq_nat
+--def beq_ident := beq_nat
+instance : decidable_eq ident :=
+by unfold ident; apply_instance
 
-theorem beq_nat00 : beq_nat 0 0 = tt := rfl.
+--theorem beq_nat00 : beq_nat 0 0 = tt := rfl.
 
-theorem beq_refl (n : ℕ) : beq_nat n n=tt :=
-begin
-    induction n, rewrite beq_nat00,
+--theorem beq_refl (n : ℕ) : beq_nat n n=tt :=
+--begin
+--    induction n, rewrite beq_nat00,
+--
+--    unfold beq_nat, rewrite n_ih
+--end
 
-    unfold beq_nat, rewrite n_ih
-end
 
-
-theorem beq_nat_comm (a : ℕ) : ∀ b, beq_nat a b=beq_nat b a := begin
-    induction a, intro b, destruct b, intro, rewrite a,
-    intro, intro, rewrite a, unfold beq_nat,
-
-    intro b, destruct b, intro, rewrite a, unfold beq_nat,
-
-    intro, intro, rewrite a, unfold beq_nat, rewrite a_ih
-end
+--theorem beq_nat_comm (a : ℕ) : ∀ b, beq_nat a b=beq_nat b a := begin
+--    induction a, intro b, destruct b, intro, rewrite a,
+--    intro, intro, rewrite a, unfold beq_nat,
+--
+--    intro b, destruct b, intro, rewrite a, unfold beq_nat,
+--
+--    intro, intro, rewrite a, unfold beq_nat, rewrite a_ih
+--end
 
 def override (st : env) (v : ident) (n : ℕ) : env :=
-    (λ (l : ident), if beq_nat v l then n else (st l))
+    (λ (l : ident), if v=l then n else (st l))
 
 theorem override_eq (n : ℕ) (V : ident) (st : env) : (override st V n) V=n :=
 begin
-    unfold override,
-    rewrite beq_refl,
-    simp
+    unfold override, simp
 end
 
 theorem override_neq (n : ℕ) (V1 : ident) (V2 : ident) (st : env) :
-    beq_ident V2 V1=ff →
+    V2 ≠ V1 →
     (override st V2 n) V1=st V1 := begin
-    unfold override, unfold beq_ident, intro, rewrite a,
-    simp
+    unfold override, intro, simp *
 end
 
 theorem override_shadow (x1 : ℕ) (x2 : ℕ) (k : ident) (f : env) :
    (override (override f k x1) k x2) = (override f k x2) :=
 begin
-    unfold override, apply funext, intro, destruct (beq_nat k x),
-    intro,rewrite a,simp,intro,rewrite a,simp
+    unfold override, funext, by_cases (k=l), simp *,
+    simp *
 end
 
-theorem beq_nat_eq (a : ℕ) : ∀ b, beq_nat a b=tt → a=b :=
-begin
-    induction a,
-    intro b,
-    destruct b, intro, rewrite a, unfold beq_nat, intro, reflexivity,
-    intro, intro, rewrite a, unfold beq_nat, simp,
-
-    intro b, destruct b, intro, rewrite a, unfold beq_nat, simp,
-    intro, intro, rewrite a, simp, unfold beq_nat,
-    intro, apply a_ih, apply a_1
-end
+--theorem beq_nat_eq (a : ℕ) : ∀ b, beq_nat a b=tt → a=b :=
+--begin
+--    induction a,
+--    intro b,
+--    destruct b, intro, rewrite a, unfold beq_nat, intro, reflexivity,
+--    intro, intro, rewrite a, unfold beq_nat, simp,
+--
+--    intro b, destruct b, intro, rewrite a, unfold beq_nat, simp,
+--    intro, intro, rewrite a, simp, unfold beq_nat,
+--    intro, apply a_ih, apply a_1
+--end
 
 theorem override_same (x1 : ℕ) (k1 : ident) (k2 : ident) (f : env) :
   f k1 = x1 →
   (override f k1 x1) k2 = f k2 :=
 begin
-    intro, unfold override, destruct (beq_nat k1 k2), intro,
-    rewrite a_1, simp, intro, rewrite a_1, simp,
-    have ek : k1=k2, apply beq_nat_eq, exact a_1,
-    subst k1, rewrite a
+    intro, unfold override, by_cases (k1=k2),
+    simp *, rw ← a, rw h,
+    simp *
 end
 
 /---------------------------------------------------------------------------/
 
 inductive aexp : Type
-  | ANum : ℕ → aexp
-  | AVar : ident → aexp
-  | APlus : aexp → aexp → aexp
-  | AMinus : aexp → aexp → aexp
-  | AMult : aexp → aexp → aexp
-  | AEq : aexp → aexp → aexp
-  | ALe : aexp → aexp → aexp
-  | ALand : aexp → aexp → aexp
-  | ALor : aexp → aexp → aexp
-  | ALnot : aexp → aexp
+  | Num : ℕ → aexp
+  | Var : ident → aexp
+  | Plus : aexp → aexp → aexp
+  | Minus : aexp → aexp → aexp
+  | Mult : aexp → aexp → aexp
+  | Eq : aexp → aexp → aexp
+  | Le : aexp → aexp → aexp
+  | Land : aexp → aexp → aexp
+  | Lor : aexp → aexp → aexp
+  | Lnot : aexp → aexp
 
 -- Shorthand for common nats and nat operators
 
-def A0 := (aexp.ANum 0)
-def A1 := (aexp.ANum 1)
-def A2 := (aexp.ANum 2)
-def A3 := (aexp.ANum 3)
-def A4 := (aexp.ANum 4)
-def A5 := (aexp.ANum 5)
-def A6 := (aexp.ANum 6)
+def A0 := (aexp.Num 0)
+def A1 := (aexp.Num 1)
+def A2 := (aexp.Num 2)
+def A3 := (aexp.Num 3)
+def A4 := (aexp.Num 4)
+def A5 := (aexp.Num 5)
+def A6 := (aexp.Num 6)
 
 infix `***`:50 := aexp.AMult
 
@@ -148,19 +148,19 @@ definition Z := 2
 --com is intended to mimic the constructs of a statement block in C or C++.
 
 inductive com : Type
-  | CSkip : com
-  | CLoad : ident -> aexp -> com
-  | CStore : aexp -> aexp -> com
-  | CAss : ident -> aexp -> com
-  | CNew : ident -> aexp -> com
-  | CDelete: aexp -> aexp -> com
-  | CSeq : com -> com -> com
-  | CIf : aexp -> com -> com -> com
-  | CWhile : aexp -> com -> com
-  | CCall : ident -> ident -> (list aexp) -> com
-  | CReturn : aexp -> com
-  | CThrow : ident -> aexp -> com
-  | CCatch : ident -> ident -> com -> com -> com.
+  | Skip : com
+  | Load : ident -> aexp -> com
+  | Store : aexp -> aexp -> com
+  | Ass : ident -> aexp -> com
+  | New : ident -> aexp -> com
+  | Delete: aexp -> aexp -> com
+  | Seq : com -> com -> com
+  | If : aexp -> com -> com -> com
+  | While : aexp -> com -> com
+  | Call : ident -> ident -> (list aexp) -> com
+  | Return : aexp -> com
+  | Throw : ident -> aexp -> com
+  | Catch : ident -> ident -> com -> com -> com.
 
 notation  `SKIP` := com.CSkip.
 infix `;` := com.CSeq.
@@ -186,16 +186,16 @@ def v_or_z : option ℕ → ℕ
 | (option.some x) := x
 
 def aeval : env → aexp → ℕ 
-  | e (aexp.ANum n) := n
-  | e (aexp.AVar ii) := e ii
-  | e (aexp.APlus a1 a2) := (aeval e a1)+(aeval e a2)
-  | e (aexp.AMinus a1 a2) := (aeval e a1)-(aeval e a2)
-  | e (aexp.AMult a1 a2) := (aeval e a1)*(aeval e a2)
-  | e (aexp.AEq a1 a2) := if beq_nat (aeval e a1) (aeval e a2) then 1 else 0
-  | e (aexp.ALe a1 a2) := if ble_nat (aeval e a1) (aeval e a2) then 1 else 0
-  | e (aexp.ALnot a1) := if beq_nat (aeval e a1) 0 then 1 else 0
-  | e (aexp.ALand a1 a2) := if beq_nat (aeval e a1) 0 then 0 else aeval e a2
-  | e (aexp.ALor a1 a2) := if beq_nat (aeval e a1) 0 then aeval e a2 else (aeval e a1)
+  | e (aexp.Num n) := n
+  | e (aexp.Var ii) := e ii
+  | e (aexp.Plus a1 a2) := (aeval e a1)+(aeval e a2)
+  | e (aexp.Minus a1 a2) := (aeval e a1)-(aeval e a2)
+  | e (aexp.Mult a1 a2) := (aeval e a1)*(aeval e a2)
+  | e (aexp.Eq a1 a2) := if (aeval e a1)=(aeval e a2) then 1 else 0
+  | e (aexp.Le a1 a2) := if (aeval e a1)≤(aeval e a2) then 1 else 0
+  | e (aexp.Lnot a1) := if (aeval e a1)=0 then 1 else 0
+  | e (aexp.Land a1 a2) := if (aeval e a1)=0 then 0 else aeval e a2
+  | e (aexp.Lor a1 a2) := if (aeval e a1)=0 then aeval e a2 else (aeval e a1)
 
 def aeval_list : env → (list aexp) → list nat
 | s list.nil := list.nil
@@ -203,36 +203,36 @@ def aeval_list : env → (list aexp) → list nat
 
 -- Auxilliary functions needed for the evaluation relation
 
-def bind_option {X : Type} {Y : Type} :
-option X → (X → option Y)
-→ option Y
-| none f := none
-| (some x) f := f x
+--def bind_option {X : Type} {Y : Type} :
+--option X → (X → option Y)
+--→ option Y
+--| none f := none
+--| (some x) f := f x
 
 --Implicit Arguments bind_option [X Y].
 
 
 def range : ℕ → ℕ → ℕ → bool
 | start 0 n := ff
-| start (s+1) t := if beq_nat t (start+s) then tt
+| start (s+1) t := if t=(start+s) then tt
                    else range start s t
 
-inductive new_heap_cells : heap -> nat -> nat -> heap -> Prop
+inductive new_heap_cells : heap → nat → nat → heap → Prop
 | OHDone : ∀ h, ∀ v,
            new_heap_cells h v 0 h
 | OHNext : ∀ h h' v c h'' val,
              new_heap_cells h (v+1) c h' →
              h' v = option.none →
-             h'' = (λ x, if beq_nat x v then option.some val
+             h'' = (λ x, if x=v then option.some val
                          else h' x) →
              new_heap_cells h v (c+1) h''
 
-inductive clear_heap_cells : heap -> nat -> nat -> heap -> Prop
+inductive clear_heap_cells : heap → nat → nat → heap → Prop
 | CHDone : ∀ h v, clear_heap_cells h v 0 h
 | CHNext : ∀ h h' v c val h'',
            clear_heap_cells h (v+1) c h' →
            h' v = option.some val →
-           h'' = (λ x, if beq_nat x v then option.none else h' x) →
+           h'' = (λ x, if x=v then option.none else h' x) →
            clear_heap_cells h v (c+1) h''
 
 inductive func_result : Type
@@ -244,98 +244,98 @@ def functions := ident → imp_state → (list ℕ) → imp_state →
                  func_result → Prop.
 
 inductive ceval : functions -> imp_state -> com -> imp_state -> func_result -> Prop
-| CESkip : ∀ f (st : imp_state), ceval f st com.CSkip st func_result.NoResult
-| CEAss  : ∀ f st a1 l,
-           ceval f st (com.CAss l a1) ((st.fst),(override (st.snd) l
+| Skip : ∀ f (st : imp_state), ceval f st com.Skip st func_result.NoResult
+| Ass  : ∀ f st a1 l,
+           ceval f st (com.Ass l a1) ((st.fst),(override (st.snd) l
                  (aeval st.snd a1)))
                  func_result.NoResult
-| CENew : ∀ f (st : imp_state) l loc e count h',
-          (not (loc=0)) →
+| New : ∀ f (st : imp_state) l loc e count h',
+          loc ≠ 0 →
           count = aeval (st.snd) e →
           new_heap_cells (st.fst) loc count h' →
-          ceval f st (com.CNew l e) (h',override (st.snd) l loc)
+          ceval f st (com.New l e) (h',override (st.snd) l loc)
                 func_result.NoResult
-| CEDelete : ∀ f (st : imp_state) loc count l c h',
+| Delete : ∀ f (st : imp_state) loc count l c h',
           l = aeval st.snd loc →
           c = aeval st.snd count →
           clear_heap_cells (st.fst) l c h' →
-          ceval f st (com.CDelete loc count) (h',st.snd)
+          ceval f st (com.Delete loc count) (h',st.snd)
                 func_result.NoResult
-| CELoad : ∀ f (st:imp_state) loc l val,
+| Load : ∀ f (st:imp_state) loc l val,
            option.some val = (st.fst) (aeval st.snd loc)  →
-           ceval f st (com.CLoad l loc)
+           ceval f st (com.Load l loc)
                  ((st.fst),(override (st.snd) l val))
                  func_result.NoResult
-| CEStore : ∀ f (st : imp_state) loc val l v ov,
+| Store : ∀ f (st : imp_state) loc val l v ov,
       v = aeval st.snd val →
       l = aeval st.snd loc →
       (st.fst) l = option.some ov →
-      ceval f st (com.CStore loc val)
-            ((λ x, if beq_nat l x then (option.some v) else (st.fst) x),(st.snd)) func_result.NoResult
-| CESeq1 : ∀ f c1 c2 st st' st'' r,
+      ceval f st (com.Store loc val)
+            ((λ x, if l=x then (option.some v) else (st.fst) x),(st.snd)) func_result.NoResult
+| Seq1 : ∀ f c1 c2 st st' st'' r,
       ceval f st c1 st' func_result.NoResult →
       ceval f st' c2 st'' r →
-      ceval f st (com.CSeq c1 c2) st'' r
-| CESeq2 : ∀ f c1 c2 st st' v,
+      ceval f st (com.Seq c1 c2) st'' r
+| Seq2 : ∀ f c1 c2 st st' v,
       ceval f st c1 st' (func_result.Return v) →
-      ceval f st (com.CSeq c1 c2) st' (func_result.Return v)
-| CESeq3 : ∀ f c1 c2 st st' name val,
+      ceval f st (com.Seq c1 c2) st' (func_result.Return v)
+| Seq3 : ∀ f c1 c2 st st' name val,
       ceval f st c1 st' (func_result.Exception name val) →
-      ceval f st (com.CSeq c1 c2) st'
+      ceval f st (com.Seq c1 c2) st'
             (func_result.Exception name val)
-| CEIfTrue : ∀ f r (st : imp_state) (st':imp_state) b1 c1 c2,
+| IfTrue : ∀ f r (st : imp_state) (st':imp_state) b1 c1 c2,
       not(aeval st.snd b1 = 0) ->
       ceval f st c1 st' r ->
-      ceval f st (com.CIf b1 c1 c2) st' r
-| CEIfFalse : ∀ f r (st : imp_state) (st' : imp_state) b1 c1 c2,
+      ceval f st (com.If b1 c1 c2) st' r
+| IfFalse : ∀ f r (st : imp_state) (st' : imp_state) b1 c1 c2,
       aeval st.snd b1 = 0 →
       ceval f st c2 st' r →
-      ceval f st (com.CIf b1 c1 c2) st' r
-| CEWhileEnd : ∀ f b1 (st : imp_state) c1,
+      ceval f st (com.If b1 c1 c2) st' r
+| WhileEnd : ∀ f b1 (st : imp_state) c1,
       aeval st.snd b1 = 0 →
-      ceval f st (com.CWhile b1 c1) st func_result.NoResult
-| CEWhileLoop1 : ∀ f (st : imp_state) st' st'' b1 c1 r,
+      ceval f st (com.While b1 c1) st func_result.NoResult
+| WhileLoop1 : ∀ f (st : imp_state) st' st'' b1 c1 r,
       not(aeval st.snd b1 = 0) →
       ceval f st c1 st' func_result.NoResult →
-      ceval f st' (com.CWhile b1 c1) st'' r →
-      ceval f st (com.CWhile b1 c1) st'' r
-| CEWhileLoop2 : ∀ f (st : imp_state) st' b1 c1 r,
+      ceval f st' (com.While b1 c1) st'' r →
+      ceval f st (com.While b1 c1) st'' r
+| WhileLoop2 : ∀ f (st : imp_state) st' b1 c1 r,
       not(aeval st.snd b1 = 0) →
       ceval f st c1 st' (func_result.Return r) →
-      ceval f st (com.CWhile b1 c1) st' (func_result.Return r)
-| CEWhileLoop3 : ∀ f (st : imp_state) st' b1 c1 name val,
+      ceval f st (com.While b1 c1) st' (func_result.Return r)
+| WhileLoop3 : ∀ f (st : imp_state) st' b1 c1 name val,
       not(aeval st.snd b1 = 0) →
       ceval f st c1 st' (func_result.Exception name val) →
-      ceval f st (com.CWhile b1 c1) st'
+      ceval f st (com.While b1 c1) st'
             (func_result.Exception name val)
-| CEThrow: ∀ f (st : imp_state) val exp v,
+| Throw: ∀ f (st : imp_state) val exp v,
       val = aeval st.snd exp ->
-      ceval f st (com.CThrow v exp) st (func_result.Exception v val)
-| CECatch1: ∀ f st st' exc var code hand,
+      ceval f st (com.Throw v exp) st (func_result.Exception v val)
+| Catch1: ∀ f st st' exc var code hand,
       ceval f st code st' func_result.NoResult →
-      ceval f st (com.CCatch exc var code hand) st' func_result.NoResult
-| CECatch2: ∀ f st st' exc var code hand v,
+      ceval f st (com.Catch exc var code hand) st' func_result.NoResult
+| Catch2: ∀ f st st' exc var code hand v,
       ceval f st code st' (func_result.Return v) →
-      ceval f st (com.CCatch exc var code hand) st' (func_result.Return v)
-| CECatch3: ∀ f st st' exc var code hand v name,
+      ceval f st (com.Catch exc var code hand) st' (func_result.Return v)
+| Catch3: ∀ f st st' exc var code hand v name,
       ceval f st code st' (func_result.Exception name v) →
       name ≠ exc →
-      ceval f st (com.CCatch exc var code hand) st'
+      ceval f st (com.Catch exc var code hand) st'
             (func_result.Exception name v)
-| CECatch4: ∀ f st st' exc var code hand v st'' name r,
+| Catch4: ∀ f st st' exc var code hand v st'' name r,
       ceval f st code st' (func_result.Exception exc v) →
       ceval f ((st'.fst),override (st'.snd) var v) hand st'' r →
       name ≠ exc →
-      ceval f st (com.CCatch exc var code hand) st'' r
-| CECall1: ∀ vl (st : imp_state) el (f:functions) (st':imp_state) r (fid:ident) var,
+      ceval f st (com.Catch exc var code hand) st'' r
+| Call1: ∀ vl (st : imp_state) el (f:functions) (st':imp_state) r (fid:ident) var,
       vl = aeval_list st.snd el →
       f fid st vl st' (func_result.Return r) →
-      ceval f st (com.CCall var fid el) ((st'.fst),override (st'.snd) var r)
+      ceval f st (com.Call var fid el) ((st'.fst),override (st'.snd) var r)
             func_result.NoResult
-| CECall2: ∀ vl (st : imp_state) el (f:functions) (st':imp_state) r (fid:ident) var name,
+| Call2: ∀ vl (st : imp_state) el (f:functions) (st':imp_state) r (fid:ident) var name,
       vl = aeval_list st.snd el →
       f fid st vl st' (func_result.Exception name r) →
-      ceval f st (com.CCall var fid el) st' (func_result.Exception name r).
+      ceval f st (com.Call var fid el) st' (func_result.Exception name r).
 
 
 
